mem/Mem1.v
@@ -92,35 +92,59 @@ Section PROOF.
              (fun _ => trigger (Choose _))
   .
 
-  Definition MemStb: list (fname * funspec) :=
+  Definition MemStb: list (fname * fspec) :=
   [("alloc", mk "Mem"
                (fun sz varg _ => varg = [Vint (Z.of_nat sz)])
                (fun sz vret rret =>
                   exists b, vret = Vptr b 0 /\
                             rret = GRA.padding (fold_left URA.add
                                                           (mapi (fun n _ => (b, Z.of_nat n) |-> (Vint 0))
-                                                                (List.repeat tt sz)) URA.unit))
-               (fun _ => trigger (Choose _))) ;
+                                                                (List.repeat tt sz)) URA.unit))) ;
   ("free", mk "Mem"
               (fun '(b, ofs, v) varg rarg => varg = [Vptr b ofs] /\
                                              rarg = (GRA.padding ((b, ofs) |-> v)))
-              (top3)
-              (fun _ => trigger (Choose _))) ;
+              (top3)) ;
   ("load", mk "Mem"
               (fun '(b, ofs, v) varg rarg => varg = [Vptr b ofs] /\
                                              rarg = (GRA.padding ((b, ofs) |-> v)))
-              (fun '(b, ofs, v) vret rret => rret = (GRA.padding ((b, ofs) |-> v)) /\ vret = v)
-              (fun _ => trigger (Choose _))) ;
+              (fun '(b, ofs, v) vret rret => rret = (GRA.padding ((b, ofs) |-> v)) /\ vret = v)) ;
   ("store", mk "Mem"
                (fun '(b, ofs, v_old, v_new) varg rarg =>
                   varg = [Vptr b ofs ; v_new] /\ rarg = (GRA.padding ((b, ofs) |-> v_old)))
-               (fun '(b, ofs, v_old, v_new) _ rret => rret = (GRA.padding ((b, ofs) |-> v_new)))
-               (fun _ => trigger (Choose _)))
+               (fun '(b, ofs, v_old, v_new) _ rret => rret = (GRA.padding ((b, ofs) |-> v_new))))
   ]
   .
 
+  Definition MemFtb: list (fname * fspec * (list val -> itree (hCallE +' eventE) val)) :=
+    zip pair MemStb (List.repeat (fun _ => trigger (Choose _)) 4)
+  .
+
+  (* Definition MemFtb2: list (fname * fspec * (list val -> itree (hCallE +' eventE) val)) := *)
+  (* [("alloc", mk "Mem" *)
+  (*              (fun sz varg _ => varg = [Vint (Z.of_nat sz)]) *)
+  (*              (fun sz vret rret => *)
+  (*                 exists b, vret = Vptr b 0 /\ *)
+  (*                           rret = GRA.padding (fold_left URA.add *)
+  (*                                                         (mapi (fun n _ => (b, Z.of_nat n) |-> (Vint 0)) *)
+  (*                                                               (List.repeat tt sz)) URA.unit)), (fun _ => trigger (Choose _))) ; *)
+  (* ("free", mk "Mem" *)
+  (*             (fun '(b, ofs, v) varg rarg => varg = [Vptr b ofs] /\ *)
+  (*                                            rarg = (GRA.padding ((b, ofs) |-> v))) *)
+  (*             (top3), (fun _ => trigger (Choose _))) ; *)
+  (* ("load", mk "Mem" *)
+  (*             (fun '(b, ofs, v) varg rarg => varg = [Vptr b ofs] /\ *)
+  (*                                            rarg = (GRA.padding ((b, ofs) |-> v))) *)
+  (*             (fun '(b, ofs, v) vret rret => rret = (GRA.padding ((b, ofs) |-> v)) /\ vret = v), (fun _ => trigger (Choose _))) ; *)
+  (* ("store", mk "Mem" *)
+  (*              (fun '(b, ofs, v_old, v_new) varg rarg => *)
+  (*                 varg = [Vptr b ofs ; v_new] /\ rarg = (GRA.padding ((b, ofs) |-> v_old))) *)
+  (*              (fun '(b, ofs, v_old, v_new) _ rret => rret = (GRA.padding ((b, ofs) |-> v_new))), (fun _ => trigger (Choose _))) *)
+  (* ] *)
+  (* . *)
+  (* Goal MemFtb = MemFtb2. refl. Qed. *)
+
   Definition MemSem: ModSem.t := {|
-    ModSem.fnsems := List.map (map_snd (fun_to_tgt MemStb)) MemStb;
+    ModSem.fnsems := List.map (fun '(fn, fs, body) => (fn, fun_to_tgt MemStb fs body)) MemFtb;
       (* [("alloc", allocF) ; ("free", freeF) ; ("load", loadF) ; ("store", storeF)]; *)
     ModSem.initial_mrs := [("Mem", GRA.padding (URA.black (M:=_memRA) (fun _ _ => inr tt)))];
   |}
