examples/mutsum/MutF1.v
@@ -13,6 +13,13 @@ Generalizable Variables E R A B C X Y Σ.
 Set Implicit Arguments.
 
 
+Fixpoint sum (n: nat): nat :=
+  match n with
+  | O => O
+  | S m => n + sum m
+  end
+.
+Compute (sum 10).
 
 Section PROOF.
 
@@ -23,34 +30,12 @@ Section PROOF.
   Definition fBody: list val -> itree (hCallE +' eventE) val :=
     fun varg => n <- trigger (Choose _);; trigger (hCall "g" n);; trigger (Choose _)
   .
-  Definition FStb: list (fname * funspec) :=
-    [("main", mk "F" (X:=unit) top3 top3 mainBody) ;
-    ("f", mk "F" (X:=nat) () () fBody)].
-
-  (***
-        return f(10);
+  (*** TODO: it would be better if the body can depend on "X", but doing so will mandate generalization of Call.
+       related issue: https://github.com/snu-sf/rusc-program-verif/issues/48
    ***)
-  Definition mainF: list val -> itree Es val :=
-    fun _ =>
-      trigger (Call "f" [Vint 10])
-  .
-
-  (***
-    f(n) := if (n == 0) then 0 else (n + g(n-1))
-  ***)
-  Definition fF: list val -> itree Es val :=
-    fun varg =>
-      match varg with
-      | [Vint n] =>
-        if dec n 0
-        then Ret (Vint 0)
-        else m <- trigger (Call "g" [Vint (n - 1)]);; r <- (vadd (Vint n) m)?;; Ret r
-      | _ => triggerUB
-      end
-  .
-
   Definition FSem: ModSem.t := {|
-    ModSem.fnsems := [("main", mainF) ; ("f", fF)];
+    ModSem.fnsems := List.map (fun '(fn, fs, body) => (fn, fun_to_tgt GlobalStb fs body)) FFtb;
+      (* [("main", mainF) ; ("f", fF)]; *)
     ModSem.initial_mrs := [("F", ε)];
   |}
   .
