examples/mutsum/MutHeader.v
@@ -1,0 +1,34 @@
+Require Import Coqlib.
+Require Import ITreelib.
+Require Import Universe.
+Require Import STS.
+Require Import Behavior.
+Require Import ModSem.
+Require Import Skeleton.
+Require Import PCM.
+Require Import Hoare.
+
+Generalizable Variables E R A B C X Y Σ.
+
+Set Implicit Arguments.
+
+
+Fixpoint sum (n: nat): nat :=
+  match n with
+  | O => O
+  | S m => n + sum m
+  end
+.
+Compute (sum 10).
+
+Section PROOF.
+
+  Context `{Σ: GRA.t}.
+
+  Definition GlobalStb: list (fname * fspec) := [
+    ("main", mk "F" (X:=unit) top3 top3) ;
+    ("f", mk "F" (X:=nat) (fun n varg _ => varg = [Vint (Z.of_nat n)]) (fun n vret _ => vret = Vint (Z.of_nat (sum n)))) ;
+    ("g", mk "F" (X:=nat) (fun n varg _ => varg = [Vint (Z.of_nat n)]) (fun n vret _ => vret = Vint (Z.of_nat (sum n))))
+  ].
+
+End PROOF.
